
\documentclass[11pt,a4paper]{article}
\usepackage{amsmath,amsthm}

\newcommand{\fn}[1]{{\tt #1}}
\newcommand{\cn}[1]{{\tt \char"5C #1}}

\title{
"}\n\n\\begin{document}\n\n\\maketitle\n\n"
f(x) = (x^3 + 2x)e^x

y = \frac{x^3}{1 - x^2}

f(x) = 3x^2 - 2 cos x

\frac{3\pi, 2}

 F(x) = (x^4 + 3x^2 - 2)^5

 y = (2x - 5)^4(8x^2 - 5)^{-3}

 x^3 + y^3 = 1

 e^y cos x = 1 + sin(xy)

 f(x) = sin(ln x)

 y = ln(e^{-x} + xe^{-x})

f(x) = (x^3 + 2x)e^x

y = \frac{x^3}{1 - x^2}

f(x) = 3x^2 - 2 cos x

\frac{3\pi, 2}

 F(x) = (x^4 + 3x^2 - 2)^5

 y = (2x - 5)^4(8x^2 - 5)^{-3}

 x^3 + y^3 = 1

 e^y cos x = 1 + sin(xy)

 f(x) = sin(ln x)

 y = ln(e^{-x} + xe^{-x})

f(x) = (x^3 + 2x)e^x

y = \frac{x^3}{1 - x^2}

f(x) = 3x^2 - 2 cos x

\frac{3\pi, 2}

 F(x) = (x^4 + 3x^2 - 2)^5

 y = (2x - 5)^4(8x^2 - 5)^{-3}

 x^3 + y^3 = 1

 e^y cos x = 1 + sin(xy)

 f(x) = sin(ln x)

 y = ln(e^{-x} + xe^{-x})

f(x) = (x^3 + 2x)e^x

y = \frac{x^3}{1 - x^2}

f(x) = 3x^2 - 2 cos x

\frac{3\pi, 2}

 F(x) = (x^4 + 3x^2 - 2)^5

 y = (2x - 5)^4(8x^2 - 5)^{-3}

 x^3 + y^3 = 1

 e^y cos x = 1 + sin(xy)

 f(x) = sin(ln x)

 y = ln(e^{-x} + xe^{-x})

f(x) = (x^3 + 2x)e^x

y = \frac{x^3}{1 - x^2}

f(x) = 3x^2 - 2 cos x

\frac{3\pi, 2}

 F(x) = (x^4 + 3x^2 - 2)^5

 y = (2x - 5)^4(8x^2 - 5)^{-3}

 x^3 + y^3 = 1

 e^y cos x = 1 + sin(xy)

 f(x) = sin(ln x)

 y = ln(e^{-x} + xe^{-x})

f(x) = (x^3 + 2x)e^x

y = \frac{x^3}{1 - x^2}

f(x) = 3x^2 - 2 cos x

\frac{3\pi, 2}

 F(x) = (x^4 + 3x^2 - 2)^5

 y = (2x - 5)^4(8x^2 - 5)^{-3}

 x^3 + y^3 = 1

 e^y cos x = 1 + sin(xy)

 f(x) = sin(ln x)

 y = ln(e^{-x} + xe^{-x})

f(x) = (x^3 + 2x)e^x

y = \frac{x^3}{1 - x^2}

f(x) = 3x^2 - 2 cos x

\frac{3\pi, 2}

 F(x) = (x^4 + 3x^2 - 2)^5

 y = (2x - 5)^4(8x^2 - 5)^{-3}

 x^3 + y^3 = 1

 e^y cos x = 1 + sin(xy)

 f(x) = sin(ln x)

 y = ln(e^{-x} + xe^{-x})

f(x) = (x^3 + 2x)e^x

y = \frac{x^3}{1 - x^2}

f(x) = 3x^2 - 2 cos x

\frac{3\pi, 2}

 F(x) = (x^4 + 3x^2 - 2)^5

 y = (2x - 5)^4(8x^2 - 5)^{-3}

 x^3 + y^3 = 1

 e^y cos x = 1 + sin(xy)

 f(x) = sin(ln x)

 y = ln(e^{-x} + xe^{-x})

f(x) = (x^3 + 2x)e^x

y = \frac{x^3}{1 - x^2}

f(x) = 3x^2 - 2 cos x

\frac{3\pi, 2}

 F(x) = (x^4 + 3x^2 - 2)^5

 y = (2x - 5)^4(8x^2 - 5)^{-3}

 x^3 + y^3 = 1

 e^y cos x = 1 + sin(xy)

 f(x) = sin(ln x)

 y = ln(e^{-x} + xe^{-x})

y = x^{-2/5}

u = \sqrt[5]{t} + 4\sqrt{t^5}

f(x) = 3x^2 - 2 cos x

\frac{3\pi, 2}

 F(x) = (x^4 + 3x^2 - 2)^5

 y = (2x - 5)^4(8x^2 - 5)^{-3}

 x^3 + y^3 = 1

 e^y cos x = 1 + sin(xy)

 f(x) = sin(ln x)

 y = ln(e^{-x} + xe^{-x})

y = x^{-2/5}

u = \sqrt[5]{t} + 4\sqrt{t^5}

f(x) = 3x^2 - 2 cos x

\frac{3\pi, 2}

 F(x) = (x^4 + 3x^2 - 2)^5

 y = (2x - 5)^4(8x^2 - 5)^{-3}

 x^3 + y^3 = 1

 e^y cos x = 1 + sin(xy)

 f(x) = sin(ln x)

 y = ln(e^{-x} + xe^{-x})

y = x^{-2/5}

u = \sqrt[5]{t} + 4\sqrt{t^5}

f(x) = 3x^2 - 2 cos x

\frac{3\pi, 2}

 F(x) = (x^4 + 3x^2 - 2)^5

 y = (2x - 5)^4(8x^2 - 5)^{-3}

 x^3 + y^3 = 1

 e^y cos x = 1 + sin(xy)

 f(x) = sin(ln x)

 y = ln(e^{-x} + xe^{-x})

y = x^{-2/5}

u = \sqrt[5]{t} + 4\sqrt{t^5}

f(x) = 3x^2 - 2 cos x

\frac{3\pi, 2}

 F(x) = (x^4 + 3x^2 - 2)^5

 y = (2x - 5)^4(8x^2 - 5)^{-3}

 x^3 + y^3 = 1

 e^y cos x = 1 + sin(xy)

 f(x) = sin(ln x)

 y = ln(e^{-x} + xe^{-x})

y = x^{-2/5}

u = \sqrt[5]{t} + 4\sqrt{t^5}

f(x) = 3x^2 - 2 cos x

\frac{3\pi, 2}

 F(x) = (x^4 + 3x^2 - 2)^5

 y = (2x - 5)^4(8x^2 - 5)^{-3}

 x^3 + y^3 = 1

 e^y cos x = 1 + sin(xy)

 f(x) = sin(ln x)

 y = ln(e^{-x} + xe^{-x})

y = x^{-2/5}

u = \sqrt[5]{t} + 4\sqrt{t^5}

f(x) = 3x^2 - 2 cos x

\frac{3\pi, 2}

 F(x) = (x^4 + 3x^2 - 2)^5

 y = (2x - 5)^4(8x^2 - 5)^{-3}

 x^3 + y^3 = 1

 e^y cos x = 1 + sin(xy)

 f(x) = sin(ln x)

 y = ln(e^{-x} + xe^{-x})

y = x^{-2/5}

u = \sqrt[5]{t} + 4\sqrt{t^5}

f(x) = 3x^2 - 2 cos x

\frac{3\pi, 2}

 F(x) = (x^4 + 3x^2 - 2)^5

 y = (2x - 5)^4(8x^2 - 5)^{-3}

 x^3 + y^3 = 1

 e^y cos x = 1 + sin(xy)

 f(x) = sin(ln x)

 y = ln(e^{-x} + xe^{-x})

y = x^{-2/5}

u = \sqrt[5]{t} + 4\sqrt{t^5}

f(x) = 3x^2 - 2 cos x

\frac{3\pi, 2}

 F(x) = (x^4 + 3x^2 - 2)^5

 y = (2x - 5)^4(8x^2 - 5)^{-3}

 x^3 + y^3 = 1

 e^y cos x = 1 + sin(xy)

 f(x) = sin(ln x)

 y = ln(e^{-x} + xe^{-x})

y = x^{-2/5}

u = \sqrt[5]{t} + 4\sqrt{t^5}

f(x) = 3x^2 - 2 cos x

\frac{3\pi, 2}

 F(x) = (x^4 + 3x^2 - 2)^5

 y = (2x - 5)^4(8x^2 - 5)^{-3}

 x^3 + y^3 = 1

 e^y cos x = 1 + sin(xy)

 f(x) = sin(ln x)

 y = ln(e^{-x} + xe^{-x})

y = x^{-2/5}

u = \sqrt[5]{t} + 4\sqrt{t^5}

f(x) = (x^3 + 2x)e^x

y = \frac{x^3}{1 - x^2}

 F(x) = (x^4 + 3x^2 - 2)^5

 y = (2x - 5)^4(8x^2 - 5)^{-3}

 x^3 + y^3 = 1

 e^y cos x = 1 + sin(xy)

 f(x) = sin(ln x)

 y = ln(e^{-x} + xe^{-x})

y = x^{-2/5}

u = \sqrt[5]{t} + 4\sqrt{t^5}

f(x) = (x^3 + 2x)e^x

y = \frac{x^3}{1 - x^2}

 F(x) = (x^4 + 3x^2 - 2)^5

 y = (2x - 5)^4(8x^2 - 5)^{-3}

 x^3 + y^3 = 1

 e^y cos x = 1 + sin(xy)

 f(x) = sin(ln x)

 y = ln(e^{-x} + xe^{-x})

y = x^{-2/5}

u = \sqrt[5]{t} + 4\sqrt{t^5}

f(x) = (x^3 + 2x)e^x

y = \frac{x^3}{1 - x^2}

 F(x) = (x^4 + 3x^2 - 2)^5

 y = (2x - 5)^4(8x^2 - 5)^{-3}

 x^3 + y^3 = 1

 e^y cos x = 1 + sin(xy)

 f(x) = sin(ln x)

 y = ln(e^{-x} + xe^{-x})

y = x^{-2/5}

u = \sqrt[5]{t} + 4\sqrt{t^5}

f(x) = (x^3 + 2x)e^x

y = \frac{x^3}{1 - x^2}

 F(x) = (x^4 + 3x^2 - 2)^5

 y = (2x - 5)^4(8x^2 - 5)^{-3}

 x^3 + y^3 = 1

 e^y cos x = 1 + sin(xy)

 f(x) = sin(ln x)

 y = ln(e^{-x} + xe^{-x})

y = x^{-2/5}

u = \sqrt[5]{t} + 4\sqrt{t^5}

f(x) = (x^3 + 2x)e^x

y = \frac{x^3}{1 - x^2}

 F(x) = (x^4 + 3x^2 - 2)^5

 y = (2x - 5)^4(8x^2 - 5)^{-3}

 x^3 + y^3 = 1

 e^y cos x = 1 + sin(xy)

 f(x) = sin(ln x)

 y = ln(e^{-x} + xe^{-x})

y = x^{-2/5}

u = \sqrt[5]{t} + 4\sqrt{t^5}

f(x) = (x^3 + 2x)e^x

y = \frac{x^3}{1 - x^2}

 F(x) = (x^4 + 3x^2 - 2)^5

 y = (2x - 5)^4(8x^2 - 5)^{-3}

 x^3 + y^3 = 1

 e^y cos x = 1 + sin(xy)

 f(x) = sin(ln x)

 y = ln(e^{-x} + xe^{-x})

y = x^{-2/5}

u = \sqrt[5]{t} + 4\sqrt{t^5}

f(x) = (x^3 + 2x)e^x

y = \frac{x^3}{1 - x^2}

 F(x) = (x^4 + 3x^2 - 2)^5

 y = (2x - 5)^4(8x^2 - 5)^{-3}

 x^3 + y^3 = 1

 e^y cos x = 1 + sin(xy)

 f(x) = sin(ln x)

 y = ln(e^{-x} + xe^{-x})

y = x^{-2/5}

u = \sqrt[5]{t} + 4\sqrt{t^5}

f(x) = (x^3 + 2x)e^x

y = \frac{x^3}{1 - x^2}

 F(x) = (x^4 + 3x^2 - 2)^5

 y = (2x - 5)^4(8x^2 - 5)^{-3}

 x^3 + y^3 = 1

 e^y cos x = 1 + sin(xy)

 f(x) = sin(ln x)

 y = ln(e^{-x} + xe^{-x})

y = x^{-2/5}

u = \sqrt[5]{t} + 4\sqrt{t^5}

f(x) = (x^3 + 2x)e^x

y = \frac{x^3}{1 - x^2}

 F(x) = (x^4 + 3x^2 - 2)^5

 y = (2x - 5)^4(8x^2 - 5)^{-3}

 x^3 + y^3 = 1

 e^y cos x = 1 + sin(xy)

 f(x) = sin(ln x)

 y = ln(e^{-x} + xe^{-x})

y = x^{-2/5}

u = \sqrt[5]{t} + 4\sqrt{t^5}

f(x) = (x^3 + 2x)e^x

y = \frac{x^3}{1 - x^2}

f(x) = 3x^2 - 2 cos x

\frac{3\pi, 2}

 x^3 + y^3 = 1

 e^y cos x = 1 + sin(xy)

 f(x) = sin(ln x)

 y = ln(e^{-x} + xe^{-x})

y = x^{-2/5}

u = \sqrt[5]{t} + 4\sqrt{t^5}

f(x) = (x^3 + 2x)e^x

y = \frac{x^3}{1 - x^2}

f(x) = 3x^2 - 2 cos x

\frac{3\pi, 2}

 x^3 + y^3 = 1

 e^y cos x = 1 + sin(xy)

 f(x) = sin(ln x)

 y = ln(e^{-x} + xe^{-x})

y = x^{-2/5}

u = \sqrt[5]{t} + 4\sqrt{t^5}

f(x) = (x^3 + 2x)e^x

y = \frac{x^3}{1 - x^2}

f(x) = 3x^2 - 2 cos x

\frac{3\pi, 2}

 x^3 + y^3 = 1

 e^y cos x = 1 + sin(xy)

 f(x) = sin(ln x)

 y = ln(e^{-x} + xe^{-x})

y = x^{-2/5}

u = \sqrt[5]{t} + 4\sqrt{t^5}

f(x) = (x^3 + 2x)e^x

y = \frac{x^3}{1 - x^2}

f(x) = 3x^2 - 2 cos x

\frac{3\pi, 2}

 x^3 + y^3 = 1

 e^y cos x = 1 + sin(xy)

 f(x) = sin(ln x)

 y = ln(e^{-x} + xe^{-x})

y = x^{-2/5}

u = \sqrt[5]{t} + 4\sqrt{t^5}

f(x) = (x^3 + 2x)e^x

y = \frac{x^3}{1 - x^2}

f(x) = 3x^2 - 2 cos x

\frac{3\pi, 2}

 x^3 + y^3 = 1

 e^y cos x = 1 + sin(xy)

 f(x) = sin(ln x)

 y = ln(e^{-x} + xe^{-x})

y = x^{-2/5}

u = \sqrt[5]{t} + 4\sqrt{t^5}

f(x) = (x^3 + 2x)e^x

y = \frac{x^3}{1 - x^2}

f(x) = 3x^2 - 2 cos x

\frac{3\pi, 2}

 x^3 + y^3 = 1

 e^y cos x = 1 + sin(xy)

 f(x) = sin(ln x)

 y = ln(e^{-x} + xe^{-x})

y = x^{-2/5}

u = \sqrt[5]{t} + 4\sqrt{t^5}

f(x) = (x^3 + 2x)e^x

y = \frac{x^3}{1 - x^2}

f(x) = 3x^2 - 2 cos x

\frac{3\pi, 2}

 x^3 + y^3 = 1

 e^y cos x = 1 + sin(xy)

 f(x) = sin(ln x)

 y = ln(e^{-x} + xe^{-x})

y = x^{-2/5}

u = \sqrt[5]{t} + 4\sqrt{t^5}

f(x) = (x^3 + 2x)e^x

y = \frac{x^3}{1 - x^2}

f(x) = 3x^2 - 2 cos x

\frac{3\pi, 2}

 x^3 + y^3 = 1

 e^y cos x = 1 + sin(xy)

 f(x) = sin(ln x)

 y = ln(e^{-x} + xe^{-x})

y = x^{-2/5}

u = \sqrt[5]{t} + 4\sqrt{t^5}

f(x) = (x^3 + 2x)e^x

y = \frac{x^3}{1 - x^2}

f(x) = 3x^2 - 2 cos x

\frac{3\pi, 2}

 x^3 + y^3 = 1

 e^y cos x = 1 + sin(xy)

 f(x) = sin(ln x)

 y = ln(e^{-x} + xe^{-x})

y = x^{-2/5}

u = \sqrt[5]{t} + 4\sqrt{t^5}

f(x) = (x^3 + 2x)e^x

y = \frac{x^3}{1 - x^2}

f(x) = 3x^2 - 2 cos x

\frac{3\pi, 2}

 F(x) = (x^4 + 3x^2 - 2)^5

 y = (2x - 5)^4(8x^2 - 5)^{-3}

 f(x) = sin(ln x)

 y = ln(e^{-x} + xe^{-x})

y = x^{-2/5}

u = \sqrt[5]{t} + 4\sqrt{t^5}

f(x) = (x^3 + 2x)e^x

y = \frac{x^3}{1 - x^2}

f(x) = 3x^2 - 2 cos x

\frac{3\pi, 2}

 F(x) = (x^4 + 3x^2 - 2)^5

 y = (2x - 5)^4(8x^2 - 5)^{-3}

 f(x) = sin(ln x)

 y = ln(e^{-x} + xe^{-x})

y = x^{-2/5}

u = \sqrt[5]{t} + 4\sqrt{t^5}

f(x) = (x^3 + 2x)e^x

y = \frac{x^3}{1 - x^2}

f(x) = 3x^2 - 2 cos x

\frac{3\pi, 2}

 F(x) = (x^4 + 3x^2 - 2)^5

 y = (2x - 5)^4(8x^2 - 5)^{-3}

 f(x) = sin(ln x)

 y = ln(e^{-x} + xe^{-x})

y = x^{-2/5}

u = \sqrt[5]{t} + 4\sqrt{t^5}

f(x) = (x^3 + 2x)e^x

y = \frac{x^3}{1 - x^2}

f(x) = 3x^2 - 2 cos x

\frac{3\pi, 2}

 F(x) = (x^4 + 3x^2 - 2)^5

 y = (2x - 5)^4(8x^2 - 5)^{-3}

 f(x) = sin(ln x)

 y = ln(e^{-x} + xe^{-x})

y = x^{-2/5}

u = \sqrt[5]{t} + 4\sqrt{t^5}

f(x) = (x^3 + 2x)e^x

y = \frac{x^3}{1 - x^2}

f(x) = 3x^2 - 2 cos x

\frac{3\pi, 2}

 F(x) = (x^4 + 3x^2 - 2)^5

 y = (2x - 5)^4(8x^2 - 5)^{-3}

 f(x) = sin(ln x)

 y = ln(e^{-x} + xe^{-x})

y = x^{-2/5}

u = \sqrt[5]{t} + 4\sqrt{t^5}

f(x) = (x^3 + 2x)e^x

y = \frac{x^3}{1 - x^2}

f(x) = 3x^2 - 2 cos x

\frac{3\pi, 2}

 F(x) = (x^4 + 3x^2 - 2)^5

 y = (2x - 5)^4(8x^2 - 5)^{-3}

 f(x) = sin(ln x)

 y = ln(e^{-x} + xe^{-x})

y = x^{-2/5}

u = \sqrt[5]{t} + 4\sqrt{t^5}

f(x) = (x^3 + 2x)e^x

y = \frac{x^3}{1 - x^2}

f(x) = 3x^2 - 2 cos x

\frac{3\pi, 2}

 F(x) = (x^4 + 3x^2 - 2)^5

 y = (2x - 5)^4(8x^2 - 5)^{-3}

 f(x) = sin(ln x)

 y = ln(e^{-x} + xe^{-x})

y = x^{-2/5}

u = \sqrt[5]{t} + 4\sqrt{t^5}

f(x) = (x^3 + 2x)e^x

y = \frac{x^3}{1 - x^2}

f(x) = 3x^2 - 2 cos x

\frac{3\pi, 2}

 F(x) = (x^4 + 3x^2 - 2)^5

 y = (2x - 5)^4(8x^2 - 5)^{-3}

 f(x) = sin(ln x)

 y = ln(e^{-x} + xe^{-x})

y = x^{-2/5}

u = \sqrt[5]{t} + 4\sqrt{t^5}

f(x) = (x^3 + 2x)e^x

y = \frac{x^3}{1 - x^2}

f(x) = 3x^2 - 2 cos x

\frac{3\pi, 2}

 F(x) = (x^4 + 3x^2 - 2)^5

 y = (2x - 5)^4(8x^2 - 5)^{-3}

 f(x) = sin(ln x)

 y = ln(e^{-x} + xe^{-x})

y = x^{-2/5}

u = \sqrt[5]{t} + 4\sqrt{t^5}

f(x) = (x^3 + 2x)e^x

y = \frac{x^3}{1 - x^2}

f(x) = 3x^2 - 2 cos x

\frac{3\pi, 2}

 F(x) = (x^4 + 3x^2 - 2)^5

 y = (2x - 5)^4(8x^2 - 5)^{-3}

 x^3 + y^3 = 1

 e^y cos x = 1 + sin(xy)

y = x^{-2/5}

u = \sqrt[5]{t} + 4\sqrt{t^5}

f(x) = (x^3 + 2x)e^x

y = \frac{x^3}{1 - x^2}

f(x) = 3x^2 - 2 cos x

\frac{3\pi, 2}

 F(x) = (x^4 + 3x^2 - 2)^5

 y = (2x - 5)^4(8x^2 - 5)^{-3}

 x^3 + y^3 = 1

 e^y cos x = 1 + sin(xy)

y = x^{-2/5}

u = \sqrt[5]{t} + 4\sqrt{t^5}

f(x) = (x^3 + 2x)e^x

y = \frac{x^3}{1 - x^2}

f(x) = 3x^2 - 2 cos x

\frac{3\pi, 2}

 F(x) = (x^4 + 3x^2 - 2)^5

 y = (2x - 5)^4(8x^2 - 5)^{-3}

 x^3 + y^3 = 1

 e^y cos x = 1 + sin(xy)

y = x^{-2/5}

u = \sqrt[5]{t} + 4\sqrt{t^5}

f(x) = (x^3 + 2x)e^x

y = \frac{x^3}{1 - x^2}

f(x) = 3x^2 - 2 cos x

\frac{3\pi, 2}

 F(x) = (x^4 + 3x^2 - 2)^5

 y = (2x - 5)^4(8x^2 - 5)^{-3}

 x^3 + y^3 = 1

 e^y cos x = 1 + sin(xy)

y = x^{-2/5}

u = \sqrt[5]{t} + 4\sqrt{t^5}

f(x) = (x^3 + 2x)e^x

y = \frac{x^3}{1 - x^2}

f(x) = 3x^2 - 2 cos x

\frac{3\pi, 2}

 F(x) = (x^4 + 3x^2 - 2)^5

 y = (2x - 5)^4(8x^2 - 5)^{-3}

 x^3 + y^3 = 1

 e^y cos x = 1 + sin(xy)

y = x^{-2/5}

u = \sqrt[5]{t} + 4\sqrt{t^5}

f(x) = (x^3 + 2x)e^x

y = \frac{x^3}{1 - x^2}

f(x) = 3x^2 - 2 cos x

\frac{3\pi, 2}

 F(x) = (x^4 + 3x^2 - 2)^5

 y = (2x - 5)^4(8x^2 - 5)^{-3}

 x^3 + y^3 = 1

 e^y cos x = 1 + sin(xy)

y = x^{-2/5}

u = \sqrt[5]{t} + 4\sqrt{t^5}

f(x) = (x^3 + 2x)e^x

y = \frac{x^3}{1 - x^2}

f(x) = 3x^2 - 2 cos x

\frac{3\pi, 2}

 F(x) = (x^4 + 3x^2 - 2)^5

 y = (2x - 5)^4(8x^2 - 5)^{-3}

 x^3 + y^3 = 1

 e^y cos x = 1 + sin(xy)

y = x^{-2/5}

u = \sqrt[5]{t} + 4\sqrt{t^5}

f(x) = (x^3 + 2x)e^x

y = \frac{x^3}{1 - x^2}

f(x) = 3x^2 - 2 cos x

\frac{3\pi, 2}

 F(x) = (x^4 + 3x^2 - 2)^5

 y = (2x - 5)^4(8x^2 - 5)^{-3}

 x^3 + y^3 = 1

 e^y cos x = 1 + sin(xy)

y = x^{-2/5}

u = \sqrt[5]{t} + 4\sqrt{t^5}

f(x) = (x^3 + 2x)e^x

y = \frac{x^3}{1 - x^2}

f(x) = 3x^2 - 2 cos x

\frac{3\pi, 2}

 F(x) = (x^4 + 3x^2 - 2)^5

 y = (2x - 5)^4(8x^2 - 5)^{-3}

 x^3 + y^3 = 1

 e^y cos x = 1 + sin(xy)

\lim_{x \to 2} \frac{x^2 + x - 6}{x - 2}

\lim_{x \to 16} \frac{4 - \sqrt{x}}{16x - x^2}

\lim{x \to 4} \frac{5 + \sqrt{x}}{\sqrt{5 + x}}

\lim{x \to 1} e^{x^2 - x}

\lim{x \to \infty} \frac{1}{2x + 3}

\lim{x \to \infty} (\sqrt{9x^2 + x} - 3x)

f(a) = 3 - 2a + 4a^2

f(t) = 100 + 50t - 4.9t^2

\lim_{x \to 2} \frac{x^2 + x - 6}{x - 2}

\lim_{x \to 16} \frac{4 - \sqrt{x}}{16x - x^2}

\lim{x \to 4} \frac{5 + \sqrt{x}}{\sqrt{5 + x}}

\lim{x \to 1} e^{x^2 - x}

\lim{x \to \infty} \frac{1}{2x + 3}

\lim{x \to \infty} (\sqrt{9x^2 + x} - 3x)

f(a) = 3 - 2a + 4a^2

f(t) = 100 + 50t - 4.9t^2

\lim_{x \to 2} \frac{x^2 + x - 6}{x - 2}

\lim_{x \to 16} \frac{4 - \sqrt{x}}{16x - x^2}

\lim{x \to 4} \frac{5 + \sqrt{x}}{\sqrt{5 + x}}

\lim{x \to 1} e^{x^2 - x}

\lim{x \to \infty} \frac{1}{2x + 3}

\lim{x \to \infty} (\sqrt{9x^2 + x} - 3x)

f(a) = 3 - 2a + 4a^2

f(t) = 100 + 50t - 4.9t^2

\lim_{x \to 2} \frac{x^2 + x - 6}{x - 2}

\lim_{x \to 16} \frac{4 - \sqrt{x}}{16x - x^2}

\lim{x \to 4} \frac{5 + \sqrt{x}}{\sqrt{5 + x}}

\lim{x \to 1} e^{x^2 - x}

\lim{x \to \infty} \frac{1}{2x + 3}

\lim{x \to \infty} (\sqrt{9x^2 + x} - 3x)

f(a) = 3 - 2a + 4a^2

f(t) = 100 + 50t - 4.9t^2

\lim_{x \to 2} \frac{x^2 + x - 6}{x - 2}

\lim_{x \to 16} \frac{4 - \sqrt{x}}{16x - x^2}

\lim{x \to 4} \frac{5 + \sqrt{x}}{\sqrt{5 + x}}

\lim{x \to 1} e^{x^2 - x}

\lim{x \to \infty} \frac{1}{2x + 3}

\lim{x \to \infty} (\sqrt{9x^2 + x} - 3x)

f(a) = 3 - 2a + 4a^2

f(t) = 100 + 50t - 4.9t^2

\lim_{x \to 2} \frac{x^2 + x - 6}{x - 2}

\lim_{x \to 16} \frac{4 - \sqrt{x}}{16x - x^2}

\lim{x \to 4} \frac{5 + \sqrt{x}}{\sqrt{5 + x}}

\lim{x \to 1} e^{x^2 - x}

\lim{x \to \infty} \frac{1}{2x + 3}

\lim{x \to \infty} (\sqrt{9x^2 + x} - 3x)

f(a) = 3 - 2a + 4a^2

f(t) = 100 + 50t - 4.9t^2

\lim_{x \to 2} \frac{x^2 + x - 6}{x - 2}

\lim_{x \to 16} \frac{4 - \sqrt{x}}{16x - x^2}

\lim{x \to 4} \frac{5 + \sqrt{x}}{\sqrt{5 + x}}

\lim{x \to 1} e^{x^2 - x}

\lim{x \to \infty} \frac{1}{2x + 3}

\lim{x \to \infty} (\sqrt{9x^2 + x} - 3x)

f(a) = 3 - 2a + 4a^2

f(t) = 100 + 50t - 4.9t^2

\lim_{x \to 2} \frac{x^2 + x - 6}{x - 2}

\lim_{x \to 16} \frac{4 - \sqrt{x}}{16x - x^2}

\lim{x \to 4} \frac{5 + \sqrt{x}}{\sqrt{5 + x}}

\lim{x \to 1} e^{x^2 - x}

\lim{x \to \infty} \frac{1}{2x + 3}

\lim{x \to \infty} (\sqrt{9x^2 + x} - 3x)

f(a) = 3 - 2a + 4a^2

f(t) = 100 + 50t - 4.9t^2

\lim_{x \to 2} \frac{x^2 + x - 6}{x - 2}

\lim_{x \to 16} \frac{4 - \sqrt{x}}{16x - x^2}

\lim{x \to 4} \frac{5 + \sqrt{x}}{\sqrt{5 + x}}

\lim{x \to 1} e^{x^2 - x}

\lim{x \to \infty} \frac{1}{2x + 3}

\lim{x \to \infty} (\sqrt{9x^2 + x} - 3x)

f(a) = 3 - 2a + 4a^2

f(t) = 100 + 50t - 4.9t^2

\lim_{x \to -3} \frac{x + 2}{x + 3}

\lim_{x \to 2\pi^-} x csc x

\lim{x \to 4} \frac{5 + \sqrt{x}}{\sqrt{5 + x}}

\lim{x \to 1} e^{x^2 - x}

\lim{x \to \infty} \frac{1}{2x + 3}

\lim{x \to \infty} (\sqrt{9x^2 + x} - 3x)

f(a) = 3 - 2a + 4a^2

f(t) = 100 + 50t - 4.9t^2

\lim_{x \to -3} \frac{x + 2}{x + 3}

\lim_{x \to 2\pi^-} x csc x

\lim{x \to 4} \frac{5 + \sqrt{x}}{\sqrt{5 + x}}

\lim{x \to 1} e^{x^2 - x}

\lim{x \to \infty} \frac{1}{2x + 3}

\lim{x \to \infty} (\sqrt{9x^2 + x} - 3x)

f(a) = 3 - 2a + 4a^2

f(t) = 100 + 50t - 4.9t^2

\lim_{x \to -3} \frac{x + 2}{x + 3}

\lim_{x \to 2\pi^-} x csc x

\lim{x \to 4} \frac{5 + \sqrt{x}}{\sqrt{5 + x}}

\lim{x \to 1} e^{x^2 - x}

\lim{x \to \infty} \frac{1}{2x + 3}

\lim{x \to \infty} (\sqrt{9x^2 + x} - 3x)

f(a) = 3 - 2a + 4a^2

f(t) = 100 + 50t - 4.9t^2

\lim_{x \to -3} \frac{x + 2}{x + 3}

\lim_{x \to 2\pi^-} x csc x

\lim{x \to 4} \frac{5 + \sqrt{x}}{\sqrt{5 + x}}

\lim{x \to 1} e^{x^2 - x}

\lim{x \to \infty} \frac{1}{2x + 3}

\lim{x \to \infty} (\sqrt{9x^2 + x} - 3x)

f(a) = 3 - 2a + 4a^2

f(t) = 100 + 50t - 4.9t^2

\lim_{x \to -3} \frac{x + 2}{x + 3}

\lim_{x \to 2\pi^-} x csc x

\lim{x \to 4} \frac{5 + \sqrt{x}}{\sqrt{5 + x}}

\lim{x \to 1} e^{x^2 - x}

\lim{x \to \infty} \frac{1}{2x + 3}

\lim{x \to \infty} (\sqrt{9x^2 + x} - 3x)

f(a) = 3 - 2a + 4a^2

f(t) = 100 + 50t - 4.9t^2

\lim_{x \to -3} \frac{x + 2}{x + 3}

\lim_{x \to 2\pi^-} x csc x

\lim{x \to 4} \frac{5 + \sqrt{x}}{\sqrt{5 + x}}

\lim{x \to 1} e^{x^2 - x}

\lim{x \to \infty} \frac{1}{2x + 3}

\lim{x \to \infty} (\sqrt{9x^2 + x} - 3x)

f(a) = 3 - 2a + 4a^2

f(t) = 100 + 50t - 4.9t^2

\lim_{x \to -3} \frac{x + 2}{x + 3}

\lim_{x \to 2\pi^-} x csc x

\lim{x \to 4} \frac{5 + \sqrt{x}}{\sqrt{5 + x}}

\lim{x \to 1} e^{x^2 - x}

\lim{x \to \infty} \frac{1}{2x + 3}

\lim{x \to \infty} (\sqrt{9x^2 + x} - 3x)

f(a) = 3 - 2a + 4a^2

f(t) = 100 + 50t - 4.9t^2

\lim_{x \to -3} \frac{x + 2}{x + 3}

\lim_{x \to 2\pi^-} x csc x

\lim{x \to 4} \frac{5 + \sqrt{x}}{\sqrt{5 + x}}

\lim{x \to 1} e^{x^2 - x}

\lim{x \to \infty} \frac{1}{2x + 3}

\lim{x \to \infty} (\sqrt{9x^2 + x} - 3x)

f(a) = 3 - 2a + 4a^2

f(t) = 100 + 50t - 4.9t^2

\lim_{x \to -3} \frac{x + 2}{x + 3}

\lim_{x \to 2\pi^-} x csc x

\lim{x \to 4} \frac{5 + \sqrt{x}}{\sqrt{5 + x}}

\lim{x \to 1} e^{x^2 - x}

\lim{x \to \infty} \frac{1}{2x + 3}

\lim{x \to \infty} (\sqrt{9x^2 + x} - 3x)

f(a) = 3 - 2a + 4a^2

f(t) = 100 + 50t - 4.9t^2

\lim_{x \to -3} \frac{x + 2}{x + 3}

\lim_{x \to 2\pi^-} x csc x

\lim_{x \to 2} \frac{x^2 + x - 6}{x - 2}

\lim_{x \to 16} \frac{4 - \sqrt{x}}{16x - x^2}

\lim{x \to \infty} \frac{1}{2x + 3}

\lim{x \to \infty} (\sqrt{9x^2 + x} - 3x)

f(a) = 3 - 2a + 4a^2

f(t) = 100 + 50t - 4.9t^2

\lim_{x \to -3} \frac{x + 2}{x + 3}

\lim_{x \to 2\pi^-} x csc x

\lim_{x \to 2} \frac{x^2 + x - 6}{x - 2}

\lim_{x \to 16} \frac{4 - \sqrt{x}}{16x - x^2}

\lim{x \to \infty} \frac{1}{2x + 3}

\lim{x \to \infty} (\sqrt{9x^2 + x} - 3x)

f(a) = 3 - 2a + 4a^2

f(t) = 100 + 50t - 4.9t^2

\lim_{x \to -3} \frac{x + 2}{x + 3}

\lim_{x \to 2\pi^-} x csc x

\lim_{x \to 2} \frac{x^2 + x - 6}{x - 2}

\lim_{x \to 16} \frac{4 - \sqrt{x}}{16x - x^2}

\lim{x \to \infty} \frac{1}{2x + 3}

\lim{x \to \infty} (\sqrt{9x^2 + x} - 3x)

f(a) = 3 - 2a + 4a^2

f(t) = 100 + 50t - 4.9t^2

\lim_{x \to -3} \frac{x + 2}{x + 3}

\lim_{x \to 2\pi^-} x csc x

\lim_{x \to 2} \frac{x^2 + x - 6}{x - 2}

\lim_{x \to 16} \frac{4 - \sqrt{x}}{16x - x^2}

\lim{x \to \infty} \frac{1}{2x + 3}

\lim{x \to \infty} (\sqrt{9x^2 + x} - 3x)

f(a) = 3 - 2a + 4a^2

f(t) = 100 + 50t - 4.9t^2

\lim_{x \to -3} \frac{x + 2}{x + 3}

\lim_{x \to 2\pi^-} x csc x

\lim_{x \to 2} \frac{x^2 + x - 6}{x - 2}

\lim_{x \to 16} \frac{4 - \sqrt{x}}{16x - x^2}

\lim{x \to \infty} \frac{1}{2x + 3}

\lim{x \to \infty} (\sqrt{9x^2 + x} - 3x)

f(a) = 3 - 2a + 4a^2

f(t) = 100 + 50t - 4.9t^2

\lim_{x \to -3} \frac{x + 2}{x + 3}

\lim_{x \to 2\pi^-} x csc x

\lim_{x \to 2} \frac{x^2 + x - 6}{x - 2}

\lim_{x \to 16} \frac{4 - \sqrt{x}}{16x - x^2}

\lim{x \to \infty} \frac{1}{2x + 3}

\lim{x \to \infty} (\sqrt{9x^2 + x} - 3x)

f(a) = 3 - 2a + 4a^2

f(t) = 100 + 50t - 4.9t^2

\lim_{x \to -3} \frac{x + 2}{x + 3}

\lim_{x \to 2\pi^-} x csc x

\lim_{x \to 2} \frac{x^2 + x - 6}{x - 2}

\lim_{x \to 16} \frac{4 - \sqrt{x}}{16x - x^2}

\lim{x \to \infty} \frac{1}{2x + 3}

\lim{x \to \infty} (\sqrt{9x^2 + x} - 3x)

f(a) = 3 - 2a + 4a^2

f(t) = 100 + 50t - 4.9t^2

\lim_{x \to -3} \frac{x + 2}{x + 3}

\lim_{x \to 2\pi^-} x csc x

\lim_{x \to 2} \frac{x^2 + x - 6}{x - 2}

\lim_{x \to 16} \frac{4 - \sqrt{x}}{16x - x^2}

\lim{x \to \infty} \frac{1}{2x + 3}

\lim{x \to \infty} (\sqrt{9x^2 + x} - 3x)

f(a) = 3 - 2a + 4a^2

f(t) = 100 + 50t - 4.9t^2

\lim_{x \to -3} \frac{x + 2}{x + 3}

\lim_{x \to 2\pi^-} x csc x

\lim_{x \to 2} \frac{x^2 + x - 6}{x - 2}

\lim_{x \to 16} \frac{4 - \sqrt{x}}{16x - x^2}

\lim{x \to \infty} \frac{1}{2x + 3}

\lim{x \to \infty} (\sqrt{9x^2 + x} - 3x)

f(a) = 3 - 2a + 4a^2

f(t) = 100 + 50t - 4.9t^2

\lim_{x \to -3} \frac{x + 2}{x + 3}

\lim_{x \to 2\pi^-} x csc x

\lim_{x \to 2} \frac{x^2 + x - 6}{x - 2}

\lim_{x \to 16} \frac{4 - \sqrt{x}}{16x - x^2}

\lim{x \to 4} \frac{5 + \sqrt{x}}{\sqrt{5 + x}}

\lim{x \to 1} e^{x^2 - x}

f(a) = 3 - 2a + 4a^2

f(t) = 100 + 50t - 4.9t^2

\lim_{x \to -3} \frac{x + 2}{x + 3}

\lim_{x \to 2\pi^-} x csc x

\lim_{x \to 2} \frac{x^2 + x - 6}{x - 2}

\lim_{x \to 16} \frac{4 - \sqrt{x}}{16x - x^2}

\lim{x \to 4} \frac{5 + \sqrt{x}}{\sqrt{5 + x}}

\lim{x \to 1} e^{x^2 - x}

f(a) = 3 - 2a + 4a^2

f(t) = 100 + 50t - 4.9t^2

\lim_{x \to -3} \frac{x + 2}{x + 3}

\lim_{x \to 2\pi^-} x csc x

\lim_{x \to 2} \frac{x^2 + x - 6}{x - 2}

\lim_{x \to 16} \frac{4 - \sqrt{x}}{16x - x^2}

\lim{x \to 4} \frac{5 + \sqrt{x}}{\sqrt{5 + x}}

\lim{x \to 1} e^{x^2 - x}

f(a) = 3 - 2a + 4a^2

f(t) = 100 + 50t - 4.9t^2

\lim_{x \to -3} \frac{x + 2}{x + 3}

\lim_{x \to 2\pi^-} x csc x

\lim_{x \to 2} \frac{x^2 + x - 6}{x - 2}

\lim_{x \to 16} \frac{4 - \sqrt{x}}{16x - x^2}

\lim{x \to 4} \frac{5 + \sqrt{x}}{\sqrt{5 + x}}

\lim{x \to 1} e^{x^2 - x}

f(a) = 3 - 2a + 4a^2

f(t) = 100 + 50t - 4.9t^2

\lim_{x \to -3} \frac{x + 2}{x + 3}

\lim_{x \to 2\pi^-} x csc x

\lim_{x \to 2} \frac{x^2 + x - 6}{x - 2}

\lim_{x \to 16} \frac{4 - \sqrt{x}}{16x - x^2}

\lim{x \to 4} \frac{5 + \sqrt{x}}{\sqrt{5 + x}}

\lim{x \to 1} e^{x^2 - x}

f(a) = 3 - 2a + 4a^2

f(t) = 100 + 50t - 4.9t^2

\lim_{x \to -3} \frac{x + 2}{x + 3}

\lim_{x \to 2\pi^-} x csc x

\lim_{x \to 2} \frac{x^2 + x - 6}{x - 2}

\lim_{x \to 16} \frac{4 - \sqrt{x}}{16x - x^2}

\lim{x \to 4} \frac{5 + \sqrt{x}}{\sqrt{5 + x}}

\lim{x \to 1} e^{x^2 - x}

f(a) = 3 - 2a + 4a^2

f(t) = 100 + 50t - 4.9t^2

\lim_{x \to -3} \frac{x + 2}{x + 3}

\lim_{x \to 2\pi^-} x csc x

\lim_{x \to 2} \frac{x^2 + x - 6}{x - 2}

\lim_{x \to 16} \frac{4 - \sqrt{x}}{16x - x^2}

\lim{x \to 4} \frac{5 + \sqrt{x}}{\sqrt{5 + x}}

\lim{x \to 1} e^{x^2 - x}

f(a) = 3 - 2a + 4a^2

f(t) = 100 + 50t - 4.9t^2

\lim_{x \to -3} \frac{x + 2}{x + 3}

\lim_{x \to 2\pi^-} x csc x

\lim_{x \to 2} \frac{x^2 + x - 6}{x - 2}

\lim_{x \to 16} \frac{4 - \sqrt{x}}{16x - x^2}

\lim{x \to 4} \frac{5 + \sqrt{x}}{\sqrt{5 + x}}

\lim{x \to 1} e^{x^2 - x}

f(a) = 3 - 2a + 4a^2

f(t) = 100 + 50t - 4.9t^2

\lim_{x \to -3} \frac{x + 2}{x + 3}

\lim_{x \to 2\pi^-} x csc x

\lim_{x \to 2} \frac{x^2 + x - 6}{x - 2}

\lim_{x \to 16} \frac{4 - \sqrt{x}}{16x - x^2}

\lim{x \to 4} \frac{5 + \sqrt{x}}{\sqrt{5 + x}}

\lim{x \to 1} e^{x^2 - x}

f(a) = 3 - 2a + 4a^2

f(t) = 100 + 50t - 4.9t^2

\lim_{x \to -3} \frac{x + 2}{x + 3}

\lim_{x \to 2\pi^-} x csc x

\lim_{x \to 2} \frac{x^2 + x - 6}{x - 2}

\lim_{x \to 16} \frac{4 - \sqrt{x}}{16x - x^2}

\lim{x \to 4} \frac{5 + \sqrt{x}}{\sqrt{5 + x}}

\lim{x \to 1} e^{x^2 - x}

\lim{x \to \infty} \frac{1}{2x + 3}

\lim{x \to \infty} (\sqrt{9x^2 + x} - 3x)

\lim_{x \to -3} \frac{x + 2}{x + 3}

\lim_{x \to 2\pi^-} x csc x

\lim_{x \to 2} \frac{x^2 + x - 6}{x - 2}

\lim_{x \to 16} \frac{4 - \sqrt{x}}{16x - x^2}

\lim{x \to 4} \frac{5 + \sqrt{x}}{\sqrt{5 + x}}

\lim{x \to 1} e^{x^2 - x}

\lim{x \to \infty} \frac{1}{2x + 3}

\lim{x \to \infty} (\sqrt{9x^2 + x} - 3x)

\lim_{x \to -3} \frac{x + 2}{x + 3}

\lim_{x \to 2\pi^-} x csc x

\lim_{x \to 2} \frac{x^2 + x - 6}{x - 2}

\lim_{x \to 16} \frac{4 - \sqrt{x}}{16x - x^2}

\lim{x \to 4} \frac{5 + \sqrt{x}}{\sqrt{5 + x}}

\lim{x \to 1} e^{x^2 - x}

\lim{x \to \infty} \frac{1}{2x + 3}

\lim{x \to \infty} (\sqrt{9x^2 + x} - 3x)

\lim_{x \to -3} \frac{x + 2}{x + 3}

\lim_{x \to 2\pi^-} x csc x

\lim_{x \to 2} \frac{x^2 + x - 6}{x - 2}

\lim_{x \to 16} \frac{4 - \sqrt{x}}{16x - x^2}

\lim{x \to 4} \frac{5 + \sqrt{x}}{\sqrt{5 + x}}

\lim{x \to 1} e^{x^2 - x}

\lim{x \to \infty} \frac{1}{2x + 3}

\lim{x \to \infty} (\sqrt{9x^2 + x} - 3x)

\lim_{x \to -3} \frac{x + 2}{x + 3}

\lim_{x \to 2\pi^-} x csc x

\lim_{x \to 2} \frac{x^2 + x - 6}{x - 2}

\lim_{x \to 16} \frac{4 - \sqrt{x}}{16x - x^2}

\lim{x \to 4} \frac{5 + \sqrt{x}}{\sqrt{5 + x}}

\lim{x \to 1} e^{x^2 - x}

\lim{x \to \infty} \frac{1}{2x + 3}

\lim{x \to \infty} (\sqrt{9x^2 + x} - 3x)

\lim_{x \to -3} \frac{x + 2}{x + 3}

\lim_{x \to 2\pi^-} x csc x

\lim_{x \to 2} \frac{x^2 + x - 6}{x - 2}

\lim_{x \to 16} \frac{4 - \sqrt{x}}{16x - x^2}

\lim{x \to 4} \frac{5 + \sqrt{x}}{\sqrt{5 + x}}

\lim{x \to 1} e^{x^2 - x}

\lim{x \to \infty} \frac{1}{2x + 3}

\lim{x \to \infty} (\sqrt{9x^2 + x} - 3x)

\lim_{x \to -3} \frac{x + 2}{x + 3}

\lim_{x \to 2\pi^-} x csc x

\lim_{x \to 2} \frac{x^2 + x - 6}{x - 2}

\lim_{x \to 16} \frac{4 - \sqrt{x}}{16x - x^2}

\lim{x \to 4} \frac{5 + \sqrt{x}}{\sqrt{5 + x}}

\lim{x \to 1} e^{x^2 - x}

\lim{x \to \infty} \frac{1}{2x + 3}

\lim{x \to \infty} (\sqrt{9x^2 + x} - 3x)

\lim_{x \to -3} \frac{x + 2}{x + 3}

\lim_{x \to 2\pi^-} x csc x

\lim_{x \to 2} \frac{x^2 + x - 6}{x - 2}

\lim_{x \to 16} \frac{4 - \sqrt{x}}{16x - x^2}

\lim{x \to 4} \frac{5 + \sqrt{x}}{\sqrt{5 + x}}

\lim{x \to 1} e^{x^2 - x}

\lim{x \to \infty} \frac{1}{2x + 3}

\lim{x \to \infty} (\sqrt{9x^2 + x} - 3x)

\lim_{x \to -3} \frac{x + 2}{x + 3}

\lim_{x \to 2\pi^-} x csc x

\lim_{x \to 2} \frac{x^2 + x - 6}{x - 2}

\lim_{x \to 16} \frac{4 - \sqrt{x}}{16x - x^2}

\lim{x \to 4} \frac{5 + \sqrt{x}}{\sqrt{5 + x}}

\lim{x \to 1} e^{x^2 - x}

\lim{x \to \infty} \frac{1}{2x + 3}

\lim{x \to \infty} (\sqrt{9x^2 + x} - 3x)


\end{document}